Make nodup non-simp

src/llist.lean
@@ -11,16 +11,15 @@ namespace llist section
     def to_list : llist V -> list V | (P v) := [v] | (L v l) := v :: to_list l
     instance llist_to_list : has_coe (llist V) (list V) := ⟨to_list⟩
 
-    def head    :           llist V -> V       |     (P v) := v         |     (L v l) := v
-    def tail    :           llist V -> list V  |     (P v) := []        |     (L v l) := l.head :: tail l
-    def init    :           llist V -> list V  |     (P v) := []        |     (L v l) := v :: init l
-    def last    :           llist V -> V       |     (P v) := v         |     (L v l) := last l
-    def inside  :           llist V -> list V  |     (P v) := []        |     (L v l) := init l
-    def is_path :           llist V -> Prop    |     (P v) := true      |     (L v l) := adj v l.head ∧ is_path l
-    def append  :      V -> llist V -> llist V |   x (P v) := L v (P x) |   x (L v l) := L v (append x l)
-    def rev     :           llist V -> llist V |     (P v) := (P v)     |     (L v l) := append v (rev l)
-
-    @[simp] def nodup   :           llist V -> Prop    |     (P v) := true      |     (L v l) := v ∉ l ∧ nodup l
+    def head    :      llist V -> V       |   (P v) := v         |   (L v l) := v
+    def tail    :      llist V -> list V  |   (P v) := []        |   (L v l) := l.head :: tail l
+    def init    :      llist V -> list V  |   (P v) := []        |   (L v l) := v :: init l
+    def last    :      llist V -> V       |   (P v) := v         |   (L v l) := last l
+    def inside  :      llist V -> list V  |   (P v) := []        |   (L v l) := init l
+    def is_path :      llist V -> Prop    |   (P v) := true      |   (L v l) := adj v l.head ∧ is_path l
+    def append  : V -> llist V -> llist V | x (P v) := L v (P x) | x (L v l) := L v (append x l)
+    def rev     :      llist V -> llist V |   (P v) := (P v)     |   (L v l) := append v (rev l)
+    def nodup   :      llist V -> Prop    |   (P v) := true      |   (L v l) := v ∉ l ∧ nodup l
 
     @[simp] def compat (l₁ l₂ : llist V) := last l₁ = head l₂
 
@@ -44,22 +43,22 @@ namespace llist section
     @[simp] lemma concat_path (h) : is_path (concat l l' h) <-> is_path l ∧ is_path l' := by { induction l; finish [is_path] }
     @[simp] lemma mem_append      : w ∈ append v l          <-> w = v ∨ w ∈ l          := by { induction l; finish [append] }
     @[simp] lemma mem_rev         : v ∈ rev l               <-> v ∈ l                  := by { induction l; finish [rev] }
+
     @[simp] lemma mem_head        : head l ∈ l                                         := by { cases l; simp [head] }
+
     @[simp] lemma mem_last        : last l ∈ l                                         := by { induction l; finish }
 
-    @[simp] lemma append_nodup  : nodup (append x l)           <-> x ∉ l ∧ nodup l
-        := by { induction l with v v l hr; simp, simp[append], exact ne_comm, push_neg, split; rintro ⟨h1,h2⟩,
-            { have h4 := hr.mp h2, simp at h1, push_neg at h1, exact ⟨⟨h1.1 ∘ eq.symm, h4.1⟩, h1.2, h4.2⟩ },
-            { simp [append], push_neg, exact ⟨⟨h1.1 ∘ eq.symm, h2.1⟩, hr.mpr ⟨h1.2, h2.2⟩⟩ } }
+    @[simp] lemma append_nodup    : nodup (append x l)      <-> x ∉ l ∧ nodup l
+        := by { induction l; finish [append, nodup] }
 
-    @[simp] lemma append_is_path : is_path (append v l) <-> adj (last l) v ∧ is_path l
+    @[simp] lemma append_is_path  : is_path (append v l)    <-> adj (last l) v ∧ is_path l
         := by { induction l; finish [is_path, append] }
 
     @[simp] lemma rev_nodup     : nodup (rev l)                    <-> nodup l
-        := by { induction l with v v l hr; finish [rev] }
+        := by { induction l; finish [rev, nodup] }
 
     @[simp] lemma rev_is_path (h : symmetric adj) : is_path (rev l) <-> is_path l
-        := by { induction l with v v l hr; simp [rev], split; intro; finish [h a.1, is_path] }
+        := by { induction l; simp [rev, is_path], tidy }
 
     @[simp] lemma mem_concat (h) : x ∈ concat l l' h <-> x ∈ l ∨ x ∈ l'
         := by { induction l with v v l hr, refine ⟨or.inr, _⟩, simp, finish [last], finish }
@@ -67,17 +66,16 @@ namespace llist section
     @[simp] lemma concat_nil (h) : concat l (P w) h = l
         := by { induction l with v v l hr; simp *, simp at h, exact h.symm }
 
-    lemma concat_nodup (h) : nodup (concat l l' h) <-> nodup l ∧ nodup l' ∧ (∀ x, x ∈ l ∧ x ∈ l' -> x = head l') := by {
-        induction l with v v l hr; simp,
-            { tidy },
-            { rw (hr h), simp at h, refine ⟨_,_⟩,
-                { rintros ⟨h1,h2,h3,h4⟩, refine ⟨⟨_,h2⟩,h3,_⟩, finish, { rintros x h6, cases h6 with h6 h6; finish } },
-                { rintros ⟨⟨h11,h12⟩,h2,h3⟩, refine ⟨_,h12,h2,_⟩,
-                    { intro h4, apply h11, cases h4 with h5 h5,
-                        { exact h5 },
-                        { convert mem_last, have h6 := h3 v (or.inl rfl) h5, finish [last] } },
-                    { rintros x ⟨h4,h5⟩, exact h3 x (or.inr h4) h5 } } }
-    }
+    lemma concat_nodup (h) : nodup (concat l l' h) <-> nodup l ∧ nodup l' ∧ (∀ x, x ∈ l ∧ x ∈ l' -> x = head l')
+        := by { induction l with v v l hr,
+            { rw compat at h, finish [nodup, last] },
+            { simp [nodup], rw [hr h], push_neg, split,
+                { rintros ⟨⟨h1,h2⟩,h3,h4,h5⟩, refine ⟨⟨h1,h3⟩,h4,_⟩, rintros x h6, cases h6; intro h7,
+                    { subst h6, contradiction },
+                    { exact h5 x ⟨h6,h7⟩ } },
+                { rintros ⟨⟨h1,h2⟩,h3,h4⟩, refine ⟨⟨h1,_⟩,h2,h3,_⟩,
+                    { intro h5, have h6 := h4 v (or.inl rfl) h5, rw [compat,last,<-h6] at h, rw <-h at h1, exact (h1 mem_last) },
+                    { rintros x ⟨h5,h6⟩, exact h4 x (or.inr h5) h6, } } } }
 end end llist
 
 structure llist' (V : Type) (x y : V) := (l : llist V) (hx : x = l.head) (hy : l.last = y)
